Cont_Monad_Algebra.thy
@@ -92,6 +92,7 @@ definition "run f = (f (\<lambda>_. nil))"
 
 definition "check f x = f (\<lambda>P. if P then x else nil)"
 
+
 definition while' :: "(bool, 'a) cont \<Rightarrow> ('b, 'a) cont \<Rightarrow> (unit, 'a) cont"
   where "while' b m = (\<lambda>f. iter (run m); bindCont b (\<lambda>c g. if c then f () else \<bottom>) f)"
 
