sqrt_proof.thy
@@ -1,0 +1,1161 @@
+theory sqrt_proof
+imports Hoare_Logic
+begin
+
+context hoare_logic
+begin
+lemma rewrite_helper: "(\<lambda>a. (case a of (x', y) \<Rightarrow> return x') x) = (x o fst)"
+  apply (rule ext, clarsimp simp: return_def)
+  done
+
+lemma idk2: "bindCont f (\<lambda>(x', y). return x') = (\<lambda>x. f (x o fst))"
+  apply (rule ext)+
+  apply (clarsimp simp: bindCont_def return_def rewrite_helper split: prod.splits)
+  done
+
+  
+
+lemma integer_squareroot_aux_wp: "(\<And>n. hoare_triple (P n) (c n) Q) \<Longrightarrow>
+  (\<And>x y n. I x y n \<Longrightarrow> y \<noteq> 0 \<and> y \<le> y + (n div y)) \<Longrightarrow>
+ hoare_triple (\<lambda>s. I x y n \<and> (\<forall>x y . I x y n  \<longrightarrow> x \<le> y \<longrightarrow> P (x, y) s) \<and>
+   (\<forall>x y . I x y n \<longrightarrow> y < x \<longrightarrow>  I y ((y + (n div y)) div 2) n))  (do { z <- integer_squareroot_aux x y n; c z}) Q"
+  apply (rule_tac P="\<lambda>x y n. hoare_triple (\<lambda>s.  I x y n \<and>   (\<forall>x y . I x y n \<longrightarrow> x \<le> y \<longrightarrow> P (x, y) s) \<and>
+   (\<forall>x y . I x y n \<longrightarrow> y < x \<longrightarrow>  I y ((y + (n div y)) div 2) n))  (do { z <- integer_squareroot_aux x y n; c z}) Q" in
+ integer_squareroot_aux.induct[simplified]  )
+  apply (atomize)
+  apply (subst integer_squareroot_aux.simps)
+  apply (rule hoare_weaken_pre)
+   apply (wp)
+    apply (clarsimp simp: bindCont_return')
+    apply (blast)
+   apply (wp)
+   apply (erule_tac x="y + (n div y)" in allE, drule mp, clarsimp)
+  apply (assumption)
+  apply (clarsimp)
+  apply (safe; clarsimp?)
+  by (blast)
+  
+ 
+
+
+lemma "P 0 \<Longrightarrow> (\<And>n. P n \<Longrightarrow> n < n + 1 \<Longrightarrow> P (n + 1)) \<Longrightarrow> P (n :: 64 word)"
+  by (metis add.commute word_induct2 word_overflow)
+
+lemma "(2 + (n :: 64 word)) div 2 = n div 2 + 1"
+  apply (induct n rule: word_induct2; clarsimp)
+  oops
+
+
+               
+  
+definition "sqrt (n :: u64) m \<equiv> 
+  (m * m) div m = m \<and> (m * m) \<le> n \<and> 
+  (\<forall>m'. m < m' \<longrightarrow> (m' * m') div m' = m' \<longrightarrow> ( m' * m' > n))"
+
+lemma sqrt_unique: "sqrt n m \<Longrightarrow> sqrt n m' \<Longrightarrow> m = m'"
+  apply (clarsimp simp: sqrt_def)
+  apply (rule ccontr, clarsimp simp: linorder_neq_iff)
+  apply (elim disjE)
+   apply (erule_tac x=m' in allE, clarsimp) 
+   apply (fastforce)
+  apply (fastforce)
+  done
+
+lemma word_desc_induct: "P m \<Longrightarrow> (\<And>n. P n \<Longrightarrow> n \<noteq> 0 \<Longrightarrow> P (n - 1)) \<Longrightarrow> n \<le> m \<Longrightarrow> n \<noteq> 0 \<Longrightarrow> P (n :: u64)"
+  apply (erule contrapos_pp)
+  apply (induct arbitrary: n rule: word_induct2; clarsimp)
+  by (metis add_diff_cancel2 le_step_down_word)
+
+lemma "x * (x :: u64) div x = x \<Longrightarrow> x \<noteq> 0 \<Longrightarrow>  unat x * unat x < 2 ^ LENGTH(64)"
+  apply (unat_arith)
+    apply (clarsimp simp: word_arith_nat_div unat_mult_lem)
+  by (smt (verit, ccfv_SIG) div_mult_le order_le_less_trans)
+
+lemma x_square_defined_iff: "x * x div (x :: u64) = x \<longleftrightarrow> unat x * unat x < 2 ^ LENGTH(64)"
+  apply (case_tac "x=0"; clarsimp?)
+  apply (rule iffI)
+   apply (unat_arith)
+    apply (clarsimp simp: word_arith_nat_div unat_mult_lem)
+  apply (smt (verit, ccfv_SIG) div_mult_le order_le_less_trans)
+  apply (rule Word.word_div_mult)
+  using word_greater_zero_iff apply blast
+  apply (clarsimp)
+  done
+
+lemma x_squared_defined_mono: assumes x_le: "(x' :: u64) \<le> x" shows "(x * x) div x = (x :: u64) \<Longrightarrow>  x' * x' div x' = (x' :: u64)"
+  apply (clarsimp simp: x_square_defined_iff)
+  using x_le 
+  by (meson mult_le_mono order_le_less_trans word_le_nat_alt)
+
+
+lemma sqrt_iff_defined: "
+    sqrt n m \<longleftrightarrow> (m * m) div m = m \<and> m * m \<le> n \<and> (m < m + 1  \<longrightarrow> (m + 1) * (m + 1) div (m + 1) = (m + 1) \<longrightarrow>  (m + 1) * (m + 1) > n)"
+  apply (clarsimp simp: sqrt_def,safe)
+   apply (erule_tac x="m+1" in allE)
+   apply (drule mp)
+         apply (clarsimp, clarsimp)
+  using less_is_non_zero_p1 word_overflow apply blast
+  using inc_le x_squared_defined_mono apply blast
+  by (smt (verit, ccfv_SIG) inc_le mult_le_mono not_less_iff_gr_or_eq
+        order_le_less_trans unat_mult_lem word_le_nat_alt x_square_defined_iff)
+  
+  
+  
+definition "sqrt' n = (THE m. sqrt n m)"
+
+find_theorems "fst (_, _)"
+
+lemma push_res_forward: "bindCont (word_unsigned_add x y) c = (bindCont (x .+ y) (\<lambda>z. c (x + y)))"
+  apply (rule ext, clarsimp simp: bindCont_def word_unsigned_add_def Let_unfold return_def fail_def)
+  done
+
+lemma push_res_forward': 
+  "bindCont (word_unsigned_div x y) c = (bindCont (word_unsigned_div x y) (\<lambda>z. c (x div y)))"
+  apply (rule ext, clarsimp simp: bindCont_def word_unsigned_div_def Let_unfold return_def fail_def)
+  done
+
+lemma exists_singularI: "\<exists>x. P x \<Longrightarrow> \<forall>x y. P x \<longrightarrow> P y \<longrightarrow> x = y \<Longrightarrow> \<exists>!x. P x"
+  apply (clarsimp)
+  by blast
+
+lemma sqrt_eqI: "sqrt x y \<Longrightarrow> sqrt' x = y"
+  apply (clarsimp simp: sqrt'_def)
+  apply (rule the1_equality; clarsimp?)
+  apply (rule exists_singularI, blast)
+  apply (clarsimp)
+  by (simp add: sqrt_unique)
+
+
+lemma zero_sqrt_zero[simp]:  "sqrt' 0 = 0"
+  by (rule sqrt_eqI, clarsimp simp: sqrt_iff_defined)
+  apply (clarsimp simp: sqrt'_def)
+  apply (rule the_equality)
+   apply (subst sqrt_iff_defined, clarsimp)
+    apply (clarsimp)
+   apply (clarsimp simp: sqrt_def)
+   apply (clarsimp simp: sqrt_def)
+  done
+
+
+lemma one_sqrt_one:  "sqrt' 1 = (1 :: u64)"
+  by (rule sqrt_eqI, clarsimp simp: sqrt_iff_defined)
+
+
+
+lemma mul_injective: "x * 2 = y * 2 \<Longrightarrow> (x * 2) div 2 = x \<Longrightarrow> (y * 2) div 2 = y \<Longrightarrow>  (x :: u64) = y " 
+  apply (unat_arith; clarsimp)
+  done
+
+lemma div_2_times_2_div_2[simp]: "((x div 2) * 2) div 2 = ((x div 2) :: u64)"
+  by (metis (no_types, lifting) add.commute add_cancel_right_right dvd_triv_left
+               even_succ_div_2 mult.commute mult_div_mod_eq not_mod_2_eq_0_eq_1)
+
+lemma "a * x = a * y \<Longrightarrow> a \<noteq> 0 \<Longrightarrow> x = (y :: int)"
+  apply (clarsimp)
+  done
+
+
+
+lemma less_plus_1_div_two_implies_eq_1: "n \<noteq> 0 \<Longrightarrow> n \<le> (n + 1) div 2 \<Longrightarrow> (n :: u64) = 1"
+  apply (erule contrapos_pp) back
+  apply (induct n rule: word_induct2)
+   apply (clarsimp)
+  apply (clarsimp)
+  apply (unat_arith)
+  done
+
+
+
+
+lemma limited_by: "n \<ge> x \<Longrightarrow> n < n + 1 \<Longrightarrow>  x \<noteq> 0 \<Longrightarrow>  (x :: u64) + (n div x) \<le> n + 1"  
+  apply (case_tac "x = n", clarsimp)
+   apply (simp add: div_word_self)
+  oops
+  oops
+  apply (induct n arbitrary: x  rule:word_induct2; clarsimp?)
+  apply (subgoal_tac "\<exists>y. x =  y + 1", clarsimp)
+  apply (case_tac "y=0"; clarsimp?)
+   apply (drule_tac x=y in meta_spec)
+   apply (drule meta_mp)
+    apply (metis add.commute lt1_neq0 word_plus_mcs_4')
+   apply (drule meta_mp)
+    apply (metis add.commute word_overflow)
+  apply (drule meta_mp)
+    apply (clarsimp)
+  apply (uint_arith)
+    apply (safe; clarsimp?)
+  sledgehammer
+  
+  find_theorems "_ div _ \<le> _"
+
+lemma bounded_div_mono: "(x :: u64) \<le> x + y \<Longrightarrow> n \<noteq> 0 \<Longrightarrow>  x div n \<le> (x + y) div n"
+  by (simp add: div_le_mono unat_arith_simps(6) word_le_nat_alt)
+
+lemma square_less_than: "x \<le> x + n div x \<Longrightarrow> (x + n div x) div 2 = x \<Longrightarrow> x * x \<le> (n :: u64)" 
+  by (metis (no_types, lifting) add_cancel_right_right add_diff_cancel_right'
+                   div_less_dividend_word div_to_mult_word_lt mult.commute mult_2 mult_div_mod_eq
+            not_mod_2_eq_0_eq_1 one_add_one word_le_less_eq word_le_minus_one_leq word_plus_mcs_4')
+
+
+lemma square_less_than: "x \<le> x + n div x \<Longrightarrow> n \<noteq> 0 \<Longrightarrow> ((x + n div x) div 2) - 1 = x \<Longrightarrow> x * x \<le> (n :: u64)"
+  by (smt (verit, ccfv_threshold) add_diff_cancel_left'
+          diff_numeral_special(9) div_by_0_word div_lt' div_to_mult_word_lt 
+          less_1_simp linorder_not_le mult_2_right one_add_one unat_mult_lem 
+           unat_plus_simple unsigned_1 word_diff_ls'(3) word_le_less_eq word_less_div)
+  
+
+
+lemma add_galois: "z \<le> z + y \<Longrightarrow> y \<le> (x :: u64) \<Longrightarrow> x \<le> z + y \<longleftrightarrow> x - y \<le> z"
+  by (meson olen_add_eqv word_diff_ls'(3) word_diff_ls'(4))
+
+lemma times_2_cases: "2 * ((n :: u64) div 2) = n \<or> 2 * (n div 2) = (n - 1)"
+  apply (case_tac "\<exists>k. n = 2 * k", clarsimp)
+   apply (metis add.right_neutral add_diff_cancel_right' mult_div_mod_eq not_mod_2_eq_0_eq_1)
+  apply (clarsimp)
+  apply (subgoal_tac "\<exists>k. n = (2 * k) + 1")
+   apply (clarsimp)
+   apply (metis add_diff_cancel_right' even_plus_one_iff mult_div_mod_eq odd_iff_mod_2_eq_one)
+  by (meson dvdE oddE)
+
+lemma times_2_cases': "((n :: u64) div 2) * 2  = n \<or> (n div 2) * 2  = (n - 1)"
+  using times_2_cases 
+  by (simp add: mult.commute)
+
+lemma helper: " x \<noteq> 0 \<Longrightarrow> x = (n :: u64) div x \<Longrightarrow> \<exists>m\<le>x. (x * x) = n - m" 
+  apply (rule_tac x="n - (n div x * x)" in exI) 
+  apply (clarsimp)
+  apply (frule_tac f="\<lambda>n. n * x" in arg_cong)
+  apply (unat_arith, clarsimp)
+  apply (safe)
+  apply (metis (no_types, lifting) add_diff_cancel_left' mod_le_divisor mult_div_mod_eq order_le_less_trans times_div_less_eq_dividend unat_mult_lem unsigned_less)
+  using word_div_mult_le word_le_nat_alt by blast
+
+find_theorems "_ div _" "_ mod _"
+
+lemma nat_divD: " (n :: nat) div y = x \<Longrightarrow> y \<noteq> 0  \<Longrightarrow> n \<ge> x * y \<and> n \<le> y * (x + 1)"
+  apply (intro conjI)
+   apply fastforce
+  by (metis add_le_same_cancel1 div_le_mono linorder_linear nonzero_mult_div_cancel_left not_one_le_zero)
+
+
+lemmas unat_mult_simp =  unat_mult_lem[THEN iffD1]
+
+lemma unat_divD: " y \<noteq> 0 \<Longrightarrow> x \<le> x + 1 \<Longrightarrow> unat y * unat (x + 1) < 2^64 \<Longrightarrow> (n :: u64) div y = x \<Longrightarrow>
+   n \<ge> x * y \<and> n \<le> y * (x + 1)"
+  sorry
+  apply (intro context_conjI)
+  using word_div_mult_le apply blast
+  apply (clarsimp)
+  apply (unat_arith, clarsimp)
+   apply (subgoal_tac "unat y * unat (x + 1) < 2^64")
+    apply (clarsimp simp: unat_mult_simp)
+    apply (subst unat_mult_simp)
+  apply (clarsimp)
+     apply (metis unat_div word_eq_unatI)
+    apply (subst (asm) unat_mult_simp)
+  using div_lt' apply blast
+    apply (subst (asm) unat_mult_simp)
+  defer
+  
+  apply (drule nat_divD)
+  apply (insert dme)
+  apply (atomize, erule_tac x=n in allE)
+  apply (erule_tac x=y in allE; clarsimp)
+  apply (intro conjI)
+  using word_div_mult_le apply blast
+  apply (clarsimp simp: smt_arith_simplify)
+  oops
+  apply (unat_arith; clarsimp?)
+  apply (safe)
+     apply (metis mod_le_divisor mult.commute nat_add_left_cancel_le)
+  oops
+  
+
+lemma helper: " x \<noteq> 0 \<Longrightarrow> x + 2 = (n :: u64) div x \<Longrightarrow> x \<le> x + 2 \<Longrightarrow>  \<exists>m\<le>(2 * x). (x * x) = n - m" 
+  apply (case_tac "x=1"; clarsimp)
+  apply (case_tac "x=2"; clarsimp?)
+  apply (case_tac "n=9"; clarsimp?)
+
+   apply (drule unat_divD[rotated -1]; clarsimp)
+   apply (case_tac "n=8"; clarsimp?)
+  apply (case_tac "n=9"; clarsimp?)
+
+  apply (case_tac "xa=8", clarsimp)
+   apply (atomize, erule_tac x="xa - 1" in allE)
+   apply (drule mp)
+    apply (metis dual_order.refl word_coorder.extremum_unique word_leq_le_minus_one)
+   apply (drule mp)
+    defer
+    apply (clarsimp)
+  apply (case_tac "m = 4", clarsimp)
+  
+  oops
+   apply (unat_arith, clarsimp)
+ apply (rule_tac x="n - ((n div x - 2) * x)" in exI) 
+   apply (clarsimp)
+  
+  apply (intro conjI)
+   defer
+  apply (metis add_diff_cancel_right')
+    apply (clarsimp simp: smt_arith_simplify)
+  
+  apply (subgoal_tac "\<exists>k r. n = (k * x) + r \<and> r < x \<and> (k * x) div x = k \<and> unat k * unat x < 2 ^ 64", clarsimp)
+   apply (subgoal_tac "x = k - 2", clarsimp)
+    apply (clarsimp simp: smt_arith_simplify)
+    defer
+  apply (smt (verit, ccfv_threshold) add.commute diff_zero div_lt' div_mult_self1 eq_diff_eq neq_0_no_wrap unat_div unat_eq_zero unat_mult_lem unat_plus_simple word_div_lt_eq_0 word_eq_unatI word_less_def word_less_eq_iff_unsigned)
+ 
+  apply (rule_tac x="n div x" in exI)
+  apply (rule_tac x="n mod x" in exI)
+  apply (safe)
+    apply presburger
+    apply (simp add: word_greater_zero_iff word_mod_less_divisor)
+   apply (metis (mono_tags, lifting) div_lt' mult.right_neutral nonzero_mult_div_cancel_right 
+           unat_arith_simps(6) unat_eq_zero unat_mult_lem word_div_1 word_div_mult_le word_eq_unatI)
+  apply (smt (verit) Euclidean_Rings.div_eq_0_iff div_lt' eq_2_64_0 linorder_neqE_nat linorder_not_less one_div_two_eq_zero order_less_trans power_less_imp_less_exp sub_wrap word64_power_less_1' word_eq_zeroI word_le_minus_cancel word_le_minus_mono_right zero_neq_numeral)
+   apply (rule_tac x="n - ((n div x - 2) * x)" in exI) 
+  apply (clarsimp)
+  apply (intro conjI)
+    apply (clarsimp simp: smt_arith_simplify)
+
+  
+  sledgehammer
+  oops
+ (* thm word_assist
+    apply (rule word_assist, clarsimp, clarsimp)
+    apply (metis (no_types, opaque_lifting) diff_add_eq diff_diff_eq2 
+eq_iff_diff_eq_0 even_plus_one_iff inc_le plus_minus_no_overflow_ab word_div_lt_eq_0 word_div_sub word_gt_a_gt_0 word_le_less_eq word_le_not_less)
+   apply (subst (asm) div_removal'', assumption)
+  apply (clarsimp)
+  apply (simp add: olen_add_eqv)
+  apply (smt (verit) add.commute add_cancel_left_left add_cancel_right_right add_diff_cancel2 add_galois diff_add_cancel diff_diff_eq diff_diff_eq2 diff_numeral_special(9) div_less_dividend_word div_removes_mod div_word_self leD lt1_neq0 mult_2 mult_2_right mult_div_mod_eq nless_le olen_add_eqv one_add_one order_le_less_trans plus_minus_no_overflow_ab sub_wrap word_div_lt_eq_0 word_le_minus_one_leq word_sub_le_iff)
+*)  apply (rule_tac x="n div x" in exI)
+  apply (rule_tac x="n mod x" in exI)
+  apply (safe)
+    apply presburger
+    apply (simp add: word_greater_zero_iff word_mod_less_divisor)
+   apply (metis (mono_tags, lifting) div_lt' mult.right_neutral nonzero_mult_div_cancel_right 
+           unat_arith_simps(6) unat_eq_zero unat_mult_lem word_div_1 word_div_mult_le word_eq_unatI)
+  by (smt (verit) Euclidean_Rings.div_eq_0_iff div_lt' eq_2_64_0 linorder_neqE_nat linorder_not_less one_div_two_eq_zero order_less_trans power_less_imp_less_exp sub_wrap word64_power_less_1' word_eq_zeroI word_le_minus_cancel word_le_minus_mono_right zero_neq_numeral)
+
+  apply (rule_tac x="n - ((n div x - 2) * x)" in exI) 
+  apply (clarsimp)
+  apply (safe)
+   defer
+  apply (metis add_diff_cancel_right')
+  apply (frule_tac f="\<lambda>n. n * x" in arg_cong)
+  apply (unat_arith, clarsimp)
+   apply (safe)
+  sledgehammer
+  oops
+  apply (metis (no_types, lifting) add_diff_cancel_left' mod_le_divisor mult_div_mod_eq order_le_less_trans times_div_less_eq_dividend unat_mult_lem unsigned_less)
+  using word_div_mult_le word_le_nat_alt by blast
+
+
+
+lemma "y \<noteq> 0 \<Longrightarrow> (x :: u64) div y = z \<longleftrightarrow> y * z \<le> x \<and> y * (z + 1) > x"
+
+  thm 
+  apply (safe)
+    apply (metis mult.commute word_div_mult_le)
+   defer
+   apply (rule antisym)
+    apply (simp add: More_Word.word_div_mult mult.commute plus_one_helper word_greater_zero_iff)
+  
+  
+  
+
+lemma div_mod_step: "x \<le> x + r \<Longrightarrow> r < x \<Longrightarrow>  (x + r) div (x :: u64) = 1"
+  using word_div_less word_div_sub word_gt_a_gt_0 by fastforce
+
+
+
+lemma div_removes_mod: "r < x \<Longrightarrow> (k * x) \<le> ((k * x) + r) \<Longrightarrow> unat k * unat x < 2^64 \<Longrightarrow>
+  ((k * x) + r) div (x :: u64) = (k * x) div x"
+  apply (subgoal_tac "r = ((k * x) + r) mod x", clarsimp)
+   apply (smt (verit, best) add_diff_cancel_left' add_diff_cancel_right'
+   div_mult_le mod_div_mult_eq nonzero_mult_div_cancel_right not_less_iff_gr_or_eq 
+    order_le_less_trans unat_arith_simps(6) unat_eq_zero unat_mult_lem unsigned_less
+   word_eq_unatI word_gt_a_gt_0)
+  apply (unat_arith, clarsimp)
+  apply (subst unat_mult_lem[THEN iffD1])
+  apply (clarsimp simp: unat_mult_lem)
+  apply (subst msrevs(2))
+  using mod_less by presburger
+
+lemmas unat_mul_simp[simp] = unat_mult_lem[THEN iffD1]
+
+lemma div_removes_mod': "r < (x :: u64) \<Longrightarrow> x\<noteq>0  \<Longrightarrow> k * x \<le> (k * x + r) \<Longrightarrow> 
+unat k * unat x < 2 ^ 64\<Longrightarrow> 
+ ((k * x) + r) div x = k"
+  apply (subst div_removes_mod, clarsimp)
+    apply (clarsimp)
+   apply (clarsimp)
+  apply (unat_arith)
+  apply (clarsimp)
+  done
+  
+
+
+lemma "(a :: nat) \<le> b \<Longrightarrow> a \<noteq> 0 \<Longrightarrow>  (\<exists>k r. k * a + r = b \<and> r < a)"
+  apply (rule_tac x="(b div a) :: nat" in exI)
+  apply (rule_tac x="(b mod a)" in exI)
+  apply (clarsimp)
+  done
+
+  
+
+lemma word_assist: " r < k - 1 \<Longrightarrow> k \<noteq> 0 \<Longrightarrow> k \<le> k + (k - 1) \<Longrightarrow> (k :: u64) + r - 1 \<le> 2 * k - 2 " 
+  apply (rule order_trans[where y="k + (k - 1) - 1"])
+   defer
+   apply (clarsimp)
+  apply (case_tac "k \<le> k + k")
+  apply (smt (verit, ccfv_SIG) add_diff_eq diff_add_eq lt1_neq0 
+             order_trans word_diff_ls'(4) word_le_less_eq word_plus_mono_right word_random)
+  
+  by (meson Word.word_l_diffs(2) neq_0_no_wrap order_less_le plus_le_left_cancel_nowrap word_plus_mono_right2 word_sub_1_le word_sub_le_iff)
+
+
+
+lemma div_helper: "b \<noteq> 0 \<Longrightarrow>a \<le> a + b \<Longrightarrow>  a div b = (c :: u64) \<Longrightarrow> (a + b) div b = (c + 1)"
+  using div_removes_mod' 
+  by (metis (no_types, lifting) eq_diff_eq olen_add_eqv word_div_sub word_neq_0_conv)
+
+
+lemma div_removal'': "r < x \<Longrightarrow> unat k * unat x < (2^64)  \<Longrightarrow> 
+  k * x \<le> k * x + r \<Longrightarrow> (k * x + r) div x = (k :: u64)" 
+  apply (case_tac "x=0"; clarsimp)
+  apply (rule div_removes_mod')
+     apply (assumption)+
+  apply (clarsimp)
+  done
+ 
+
+lemma helper': " x \<noteq> 0 \<Longrightarrow> n \<noteq> 0 \<Longrightarrow> x \<le> n \<Longrightarrow> x * x div x = x \<Longrightarrow>  x = (n :: u64) div x - 1 \<Longrightarrow> \<exists>m\<le>(2 * x). (x * x) = n - m" 
+
+  apply (rule_tac x="n - ((n div x - 1) * x)" in exI) 
+  apply (clarsimp)
+  apply (subgoal_tac "\<exists>k r. n = (k * x) + r \<and> r < x \<and> (k * x) div x = k \<and> unat k * unat x < 2 ^ 64", clarsimp) 
+   apply (subgoal_tac "x = k - 1", clarsimp)
+    apply (clarsimp simp: smt_arith_simplify)
+    apply (rule word_assist, clarsimp, clarsimp)
+    apply (metis (no_types, opaque_lifting) diff_add_eq diff_diff_eq2 
+eq_iff_diff_eq_0 even_plus_one_iff inc_le plus_minus_no_overflow_ab word_div_lt_eq_0 word_div_sub word_gt_a_gt_0 word_le_less_eq word_le_not_less)
+   apply (subst (asm) div_removal'', assumption)
+  apply (clarsimp)
+  apply (simp add: olen_add_eqv)
+  apply (smt (verit) add.commute add_cancel_left_left add_cancel_right_right add_diff_cancel2 add_galois diff_add_cancel diff_diff_eq diff_diff_eq2 diff_numeral_special(9) div_less_dividend_word div_removes_mod div_word_self leD lt1_neq0 mult_2 mult_2_right mult_div_mod_eq nless_le olen_add_eqv one_add_one order_le_less_trans plus_minus_no_overflow_ab sub_wrap word_div_lt_eq_0 word_le_minus_one_leq word_sub_le_iff)
+  apply (rule_tac x="n div x" in exI)
+  apply (rule_tac x="n mod x" in exI)
+  apply (safe)
+    apply presburger
+    apply (simp add: word_greater_zero_iff word_mod_less_divisor)
+   apply (metis (mono_tags, lifting) div_lt' mult.right_neutral nonzero_mult_div_cancel_right 
+           unat_arith_simps(6) unat_eq_zero unat_mult_lem word_div_1 word_div_mult_le word_eq_unatI)
+  by (smt (verit) Euclidean_Rings.div_eq_0_iff div_lt' eq_2_64_0 linorder_neqE_nat linorder_not_less one_div_two_eq_zero order_less_trans power_less_imp_less_exp sub_wrap word64_power_less_1' word_eq_zeroI word_le_minus_cancel word_le_minus_mono_right zero_neq_numeral)
+
+lemma "y \<noteq> 0 \<Longrightarrow>x \<ge> y \<Longrightarrow> z \<le> x div y \<longleftrightarrow> x \<ge> z * (y :: nat)" 
+  apply (safe)
+  using td_gal apply blast
+  using less_eq_div_iff_mult_less_eq by blast
+thm th2
+
+lemma lift_div: "m \<le> n * q \<Longrightarrow> m div q \<le> (n :: nat)"
+  by (metis antisym div_by_0 linorder_linear nonzero_mult_div_cancel_right th2 zero_le)
+
+
+lemma le_div_times_iff: "unat z * unat y < 2^64 \<Longrightarrow> y \<noteq> 0 \<Longrightarrow>  x div y \<ge> z \<longleftrightarrow> x \<ge> z * (y :: u64)"
+  apply (unat_arith, clarsimp)
+  apply (safe)
+  using th2 apply blast
+  apply (subst less_eq_div_iff_mult_less_eq)
+   defer
+   apply (clarsimp)
+  apply (blast)
+  done
+
+
+lemma le_div_timesI: "x \<le> z * (y :: u64) \<Longrightarrow>  x div y \<le> z "
+  by (metis bits_div_by_0 div_lt_mult linorder_not_less word_gt_a_gt_0 word_neq_0_conv)
+
+lemma " (x + n div x) div 2 = x + 1 \<Longrightarrow> x + 2 = (n :: nat) div x \<Longrightarrow> n - x * x \<le> 2 * x" nitpick
+
+lemma square_less_than': " 2 * x + x * x \<le> 2 * x + x * x + 1 \<Longrightarrow>  2 * x \<le> 2 * x + x * x \<Longrightarrow> n \<noteq> 0 \<Longrightarrow> x \<le> x + n div x \<Longrightarrow> x \<noteq> 0 \<Longrightarrow>  (x + n div x) div 2 = x + 1 \<Longrightarrow>
+  (x + 1) * (x + 1) > (n :: nat)" 
+  apply (clarsimp simp: smt_arith_simplify) 
+  apply (subgoal_tac "n - (x * x) \<le> (2 * x)")
+  apply (smt (verit, best) add_cancel_right_left is_num_normalize(1) neq_0_no_wrap olen_add_eqv one_neq_zero plus_one_helper2 word_diff_ls'(3))
+   apply (subst add_galois)
+     defer
+  apply (simp add: square_less_than)
+  apply (assumption)
+   apply (insert times_2_cases[where n="(x + n div x)"])[1]
+  apply (elim disjE; clarsimp)
+
+  apply (rule_tac y="2 * ((x + n div x) div 2 - 1)" in  order_trans[rotated])
+    apply auto[1]
+   apply (insert times_2_cases[where n="(x + n div x)"])[1]
+  apply (elim disjE; clarsimp)
+
+  thm helper
+sledgehammer
+  oops               
+    apply (frule  helper[rotated])
+    apply (clarsimp)
+  using order_trans apply blast
+   apply (frule helper'[where x=x and n=n])
+        apply (clarsimp)
+       apply (metis add_cancel_right_right div_less_dividend_word
+             linorder_not_le one_add_one word_div_lt_eq_0 zero_neq_one)
+     apply (metis (mono_tags, lifting) add_cancel_right_right
+ antisym_conv2 div_less_dividend_word div_lt' nonzero_mult_div_cancel_right one_add_one one_neq_zero unat_0 unat_arith_simps(6) unat_mult_lem word_eq_unatI word_sub_1_le)
+     apply (assumption)
+   apply (clarsimp)
+  apply (assumption)
+  done
+
+
+  
+
+lemma square_less_than': " 2 * x + x * x \<le> 2 * x + x * x + 1 \<Longrightarrow>  2 * x \<le> 2 * x + x * x \<Longrightarrow> n \<noteq> 0 \<Longrightarrow> x \<le> x + n div x \<Longrightarrow> x \<noteq> 0 \<Longrightarrow>  (x + n div x) div 2 = x \<Longrightarrow>
+  (x + 1) * (x + 1) > (n :: u64)" 
+  apply (clarsimp simp: smt_arith_simplify) 
+  apply (subgoal_tac "n \<le> 2 * x + (x * x)")
+   apply (metis (no_types, opaque_lifting) is_num_normalize(1) lt1_neq0 olen_add_eqv plus_one_helper2)
+  apply (subgoal_tac "n - (x * x) \<le> 2 * x")
+   apply (subst add_galois)
+     defer
+  apply (metis (no_types, lifting) add.commute add_cancel_right_right div_less_dividend_word div_to_mult_word_lt mult.commute mult_2 mult_div_mod_eq neq_0_no_wrap not_mod_2_eq_0_eq_1 one_add_one plus_one_helper word_div_mult_le word_plus_mcs_4)
+    apply (assumption)
+  apply (rule_tac y="2 * ((x + n div x) div 2)" in  order_trans[rotated])
+    apply auto[1]
+   apply (insert times_2_cases[where n="(x + n div x)"])[1]
+   apply (elim disjE; clarsimp)
+    apply (frule (1) helper)
+    apply (clarsimp)
+  using order_trans apply blast
+   apply (frule helper'[where x=x and n=n])
+        apply (clarsimp)
+       apply (metis add_cancel_right_right div_less_dividend_word
+             linorder_not_le one_add_one word_div_lt_eq_0 zero_neq_one)
+     apply (metis (mono_tags, lifting) add_cancel_right_right
+ antisym_conv2 div_less_dividend_word div_lt' nonzero_mult_div_cancel_right one_add_one one_neq_zero unat_0 unat_arith_simps(6) unat_mult_lem word_eq_unatI word_sub_1_le)
+     apply (assumption)
+   apply (clarsimp)
+  apply (assumption)
+  done
+
+
+lemma context_conjI':
+  assumes Q "Q \<Longrightarrow> P"
+  shows "P \<and> Q"
+  by (iprover intro: conjI assms)
+
+lemma conjI_alt: "(P \<Longrightarrow> Q) \<Longrightarrow> (Q \<Longrightarrow> P) \<Longrightarrow> (\<not>P \<Longrightarrow> Q) \<Longrightarrow>  P \<and> Q"
+  apply (intro conjI)
+   apply (case_tac P; clarsimp)
+  apply (case_tac P; clarsimp)
+  done
+
+lemma "  x \<le> n + 1 \<Longrightarrow> n \<le> n + 1 \<Longrightarrow> (x :: 2 word) \<le> x + n div (x div 2)"  
+  oops
+  apply (induct n rule:word_induct2; clarsimp)
+  apply (drule meta_mp)
+   apply (simp add: add.commute order_le_less plus_one_helper2)
+  apply (drule meta_mp)
+   defer
+   apply (drule meta_mp)
+    defer
+   apply (drule meta_mp)
+  defer
+
+  find_consts "8 word \<Rightarrow> 16  word"
+
+  find_theorems "_ :: 'e :: len word" name:induct
+
+lemma another_helper: "
+       x \<le> n + 1 \<Longrightarrow> n < n + 1 \<Longrightarrow> 
+       x  \<le> x + ((n :: 64  word) div x)" 
+  apply (induct x rule: less_induct)
+  apply (atomize)
+  apply (case_tac "x = 0"; clarsimp)
+  apply (case_tac "x = n + 1", clarsimp)
+  apply (simp add: word_div_lt_eq_0)
+  apply (erule_tac x="x - 1" in allE)
+  apply (drule mp)
+   apply (simp add: less_1_simp)
+  apply (drule mp)
+   apply (simp add: less_1_simp word_le_less_eq)
+  by (smt (verit) add_diff_eq diff_add_eq_diff_diff_swap diff_diff_eq2 
+     div_less_dividend_word div_mod_step inc_i inc_le le_m1_iff_lt 
+      less_1_simp lt1_neq0 not_less_iff_gr_or_eq order_less_le_trans 
+       word_diff_less word_div_1 word_div_sub word_greater_zero_iff 
+      word_gt_a_gt_0 word_le_less_eq word_le_minus_one_leq word_le_not_less 
+     word_not_simps(1) word_random word_sub_le_iff word_sub_plus_one_nonzero zadd_diff_inverse)
+
+
+lemma yet_another_helper: "n div y \<le> y + 1 \<Longrightarrow> (y + n div y) div 2 \<le> (y :: u64)"
+  apply (unat_arith, clarsimp, safe; clarsimp?)
+  apply linarith
+  by (linarith)
+  by (metis div_le_dividend lift_div mult_2_right nat_add_left_cancel_le order_trans)
+
+lemma "  x \<le> n \<Longrightarrow> n div x \<le> x \<Longrightarrow>  (x + n div x) div 2 \<le> x \<Longrightarrow> n < n + 1 \<Longrightarrow> n > 4 \<Longrightarrow>
+     n div ((x + n div x) div 2) \<le>  ((x + (n :: nat) div x) div 2) + 1"
+ nitpick
+  
+  
+  
+
+lemma "(x + n div x) div 2 \<le> (x + n div x) div 2 + n div ((x + n div x) div 2) \<Longrightarrow>
+       x \<le> n + 1 \<Longrightarrow> n > 4 \<Longrightarrow> 
+       (x + n div x) div 2 \<le> x \<Longrightarrow>
+       ((x + n div x) div 2 + n div ((x + n div x) div 2)) div 2 \<le> (x + (n :: u64) div x) div 2"
+  oops
+
+lemma another_helper: "((x + n div x) div 2 + n div ((x + n div x) div 2)) div 2 \<noteq> 0 \<Longrightarrow>
+       (x + n div x) div 2 \<noteq> 0 \<Longrightarrow>
+       (x + n div x) div 2 \<le> (x + n div x) div 2 + n div ((x + n div x) div 2) \<Longrightarrow>
+       (x + n div x) div 2 \<le> x \<Longrightarrow>
+       ((x + n div x) div 2 + n div ((x + n div x) div 2)) div 2
+       \<le> ((x + n div x) div 2 + n div ((x + n div x) div 2)) div 2 +
+          (n :: 64 word) div (((x + n div x) div 2 + n div ((x + n div x) div 2)) div 2)"
+  apply (rule another_helper)
+  
+  
+  defer
+  apply (subst divide_divide_eq_right)
+  find_theorems "?x div (?y div ?z) = _"
+  oops
+  apply (induct n rule: word_bit_induct; clarsimp?)
+  sledgehammer
+  oops
+   apply (smt (z3) Orderings.order_eq_iff add.commute add_diff_cancel_left'
+  bits_div_by_1 div_word_self left_add_twice less_is_non_zero_p1 
+ linorder_le_less_linear not_less_iff_gr_or_eq one_add_one word_div_lt_eq_0 word_le_minus_one_leq)
+  by (smt (z3) add.commute add_cancel_right_right 
+               add_diff_cancel_right' bits_div_by_1 div_word_self 
+               dvd_triv_left even_succ_div_2 less_1_simp linorder_not_le mult_2 
+               not_less_iff_gr_or_eq one_add_one word_div_lt_eq_0)
+
+lemma diff_lessE: "(x :: nat) < y \<Longrightarrow> (a \<le> y \<Longrightarrow> y - a < y - x) \<Longrightarrow>  x < a"
+  apply (case_tac "a \<le> y")
+   apply (meson diff_le_mono2 le_def)
+  by auto
+
+lemma x_add_cases: "x div Suc (Suc 0) +
+        x div Suc (Suc 0) = x \<or> x div Suc (Suc 0) +
+        x div Suc (Suc 0) = (x - 1)"
+  apply (case_tac "even x"; clarsimp?)
+   apply (metis dvd_div_mult_self mult_2_right numeral_2_eq_2)
+  sorry
+  sledgehammer
+  
+
+  apply (clarsimp)
+
+  find_theorems "?x \<le> ?y \<Longrightarrow> ?x < Suc ?y" 
+
+  find_theorems name:mono "?x + ?y \<le> ?x + ?z"
+
+
+lemma midpoint_le: "x \<le> n \<Longrightarrow> (x :: nat) + n div x \<le> n + 1" 
+  apply (induct x rule: less_induct)
+  apply (case_tac x; clarsimp)
+  apply (drule_tac x=nat in meta_spec)
+  apply (clarsimp)
+  sorry
+
+lemma "x \<le> (n :: nat) \<Longrightarrow> x + 1 \<ge> (x + n div x) div 2"
+  
+lemma "Suc n \<le> x \<Longrightarrow> n < x"
+
+lemma move_it: "Suc y = x \<Longrightarrow> y \<le> a \<Longrightarrow> x \<le> Suc a"
+  by blast
+
+lemma move_it': "x = y - Suc 0 \<Longrightarrow> y \<noteq> 0 \<Longrightarrow>  x + 1 = (y :: nat)"
+  by force
+
+lemma times_2_cases_nat: "2 * ((n :: nat) div 2) = n \<or> 2 * (n div 2) = (n - 1)"
+  apply (case_tac "\<exists>k. n = 2 * k", clarsimp)
+  by (metis add.right_neutral add_diff_cancel_right' mult_div_mod_eq not_mod_2_eq_0_eq_1)
+
+
+lemma "x * (n div x) = n - n mod (x :: nat)"
+  by (metis minus_mod_eq_mult_div)
+
+lemma "z \<noteq> 0 \<Longrightarrow> (x :: nat) \<le> y div z \<longleftrightarrow> x * z \<le> y"
+  sledgehammer
+  by (simp add: less_eq_div_iff_mult_less_eq)
+
+lemma sqr_both_sides: "x * x \<le> y * y \<Longrightarrow> x \<le> (y :: nat)"
+  using mult_le_mono nat_le_linear by fastforce
+
+lemma "x \<le> n \<Longrightarrow> (x :: nat) * (n div x) = n - n mod x"
+  apply (subst minus_mod_eq_mult_div)
+lemma "m \<le> (n :: nat) \<Longrightarrow> m div x \<le> n div x"
+
+lemma "(n :: nat) div (Suc n) = 0"
+  apply (clarsimp)
+
+lemma idk: "(n :: nat) * 2 \<le> Suc n + n * n div Suc n"
+  apply (induct n; clarsimp)
+  by (simp add: less_eq_div_iff_mult_less_eq)
+
+lemma "((x :: nat) \<le> z + y) = (x - y \<le> z)"
+  sledgehammer
+  using le_diff_conv by blast
+
+lemma ratio: "p \<le> x \<Longrightarrow>  (p :: nat) * 2 \<le> x + p*p div x" 
+  apply (case_tac "x=0"; clarsimp)
+  apply (case_tac "x > 2 * p", clarsimp)
+  apply (subst add.commute)
+  apply (subst le_diff_conv[symmetric])
+  apply (subst less_eq_div_iff_mult_less_eq; clarsimp?)
+  apply (induct x; clarsimp)
+  apply (case_tac "p = Suc x", clarsimp)
+  apply (drule meta_mp, clarsimp)
+  apply (erule order_trans[rotated])
+  apply (clarsimp simp: smt_arith_simplify) 
+
+  by (smt (verit, ccfv_threshold) Suc_diff_le add.assoc add_diff_cancel_left' le_Suc_eq le_add_diff_inverse2 le_antisym le_diff_conv mult.commute mult_Suc_right nat_le_linear trans_le_add1)
+  
+  
+  apply (case_tac "n"; clarsimp)
+   
+
+lemma ge_sqrt: "(p * p) \<le> n \<Longrightarrow>  x \<ge> p \<Longrightarrow>  ((x :: nat) + n div x) div 2 \<ge> p"
+  apply (subst less_eq_div_iff_mult_less_eq)
+   apply (clarsimp)
+  apply (case_tac "x = p", clarsimp)
+   apply (metis div_by_0 div_le_mono nonzero_mult_div_cancel_right)
+  apply (clarsimp)
+  apply (rule order_trans[rotated], rule add_le_mono, rule order_refl)
+   apply (rule div_le_mono, assumption)
+  by (rule ratio, assumption)
+
+
+find_theorems name:coinduct
+
+lemma "1 + n \<noteq> 0 \<Longrightarrow>
+          m * m div m = (m :: u64) \<Longrightarrow>
+          m * m \<le> n \<Longrightarrow>
+          n \<noteq> 1 \<Longrightarrow>
+          m < m + 1 \<Longrightarrow>
+          (2 * m + (m * m + 1)) div (m + 1) = m + 1 \<Longrightarrow> n < 2 * m + (m * m + 1) \<Longrightarrow> 1 + n < 2 * m + (m * m + 1)"
+
+lemma maximal_helper: "finite S \<Longrightarrow> ((S :: u64 set) \<noteq> {}) \<Longrightarrow> \<forall>n\<in>S. n \<le> m \<Longrightarrow> \<exists>i\<in>S. \<forall>n\<in>S. i \<ge> n"
+  apply (induct S rule: finite_induct; clarsimp)
+  by (metis (no_types, lifting) empty_iff linorder_linear order_trans)
+
+lemma maximal_exists: " ((S :: u64 set) \<noteq> {}) \<Longrightarrow> \<forall>n\<in>S. n \<le> m \<Longrightarrow> \<exists>i\<in>S. \<forall>n\<in>S. i \<ge> n"
+  apply (rule maximal_helper)
+  using finite_code apply blast
+  by (auto)
+
+
+lemma (in hoare_logic) sqrt_exists_uniquely:  "\<exists>!m. (sqrt n m)"
+  apply (rule exists_singularI)
+   apply (induct n rule:word_induct2 ; clarsimp?)
+    apply (rule_tac x=0 in exI)
+    apply (clarsimp simp: sqrt_def)
+  using word_neq_0_conv apply fastforce
+   apply (case_tac "n = 0"; clarsimp?)
+    apply (rule_tac x=1 in exI)
+  apply (simp add: sqrt_iff_defined)
+   apply (insert maximal_exists[where S="{x. x * x div x = x \<and>  x * x \<le> (_ + 1)}"])
+   apply (atomize)
+  apply (erule_tac x="n" in allE)
+   apply (erule_tac x="(n + 1) div 2" in allE)
+   apply (drule mp)
+    apply (clarsimp)
+    apply (rule_tac x=0 in exI; clarsimp)
+   apply (drule mp)
+    apply (clarsimp)
+  apply (unat_arith, clarsimp)
+    defer
+    apply (clarsimp)
+    apply (rule_tac x=i in exI)
+    apply (clarsimp simp: sqrt_iff_defined)
+    apply (intro conjI; clarsimp?)
+     apply (clarsimp simp: add.commute)
+    apply (metis add.commute linorder_not_le)
+  using sqrt_unique apply presburger
+  apply (subst (asm) unat_mul_simp) back
+   apply (metis unat_div word_eq_unatI x_square_defined_iff)
+  by (smt (verit, best) One_nat_def bot_nat_0.not_eq_extremum div_le_dividend
+                        le_less_Suc_eq less_eq_div_iff_mult_less_eq linorder_le_less_linear 
+                        mult_2 mult_2_right nat.inject nat_div_eq_Suc_0_iff numeral_2_eq_2
+                        one_add_one order_le_less_trans unat_div unat_mult_lem word_eq_unatI 
+                        x_square_defined_iff zero_less_numeral)
+
+lemma (in hoare_logic) sqrt_induct: 
+  "(\<And>p. (p * p) \<le> n \<Longrightarrow> p * p div p = p \<Longrightarrow>  (p < p + 1 \<Longrightarrow> (p + 1) * (p + 1) div (p + 1) = (p + 1) \<Longrightarrow> (p + 1) * (p + 1) > n) \<Longrightarrow> P p) \<Longrightarrow>
+   P (sqrt' n)"
+  apply (clarsimp simp: sqrt'_def)
+  apply (rule the1I2)
+   apply (rule sqrt_exists_uniquely)
+  apply (clarsimp simp: sqrt_iff_defined)
+  done
+
+lemma  (in hoare_logic) word_sqrt_ge: 
+ "x \<le> x + n div x \<Longrightarrow> x \<le> n \<Longrightarrow> x \<ge> sqrt' n \<Longrightarrow> (x + n div x) div 2 \<ge> sqrt' n"
+  apply (induct rule: sqrt_induct)
+  apply (unat_arith, clarsimp)
+   apply (rule ge_sqrt)
+    apply (metis div_le_mono th2)
+   apply (assumption)
+  apply (clarsimp)
+  by (meson Nat.le_diff_conv2 div_le_dividend leD le_trans linorder_le_less_linear nat_add_left_cancel_le)
+
+
+
+lemma "x < n \<Longrightarrow>   x \<noteq> 0 \<Longrightarrow> (n :: nat) + 1 = i * i \<Longrightarrow>  
+   x = ((x +  n div x) div 2 - 1) \<Longrightarrow>
+        n < (x + 1) * (x + 1)"
+  oops
+  apply (case_tac "x \<ge> i")
+  using Suc_eq_plus1 Suc_le_lessD mult_le_mono trans_le_add1 apply presburger
+  apply (drule not_leD)
+  apply (rule Suc_le_lessD, clarsimp)
+  apply (rule move_it, assumption)
+  apply (drule move_it')
+   apply (metis One_nat_def div_2_gt_zero div_by_1 less_Suc0 
+  less_nat_zero_code linorder_neqE_nat trans_less_add1 trans_less_add2)
+  apply (drule arg_cong[where f="\<lambda>n. 2 * n"], clarsimp) back
+  apply (insert times_2_cases_nat[where n="((x + n div x))"])
+  find_theorems "2 * (?y div 2)"
+  apply (clarsimp)
+  apply (elim disjE; clarsimp?)
+   apply (drule arg_cong[where f="\<lambda>n. x * n"]) back
+   apply (subst (asm) minus_mod_eq_mult_div[symmetric]) back
+   apply (clarsimp) nitpick
+   apply (subgoal_tac "n mod x = 0", clarsimp)
+  apply (subst zmod_eq_0_iff)
+  find_theorems "?n mod ?x = 0"
+  sledgehammer
+  
+
+  
+  apply (rule order_trans[where y=" (x + n div x + x * x)"])
+  thm helper'
+  
+  oops
+  apply (induct rule: less_Suc_induct)
+   apply (clarsimp)
+   apply (smt (verit, ccfv_threshold) add.commute add_implies_diff add_le_mono1
+                                       dual_order.eq_iff le_add1 le_div_geq le_square 
+                                      less_Suc_eq mult_2 nat_div_eq_Suc_0_iff
+                                         nat_less_le not_le_imp_less numeral_2_eq_2 plus_1_eq_Suc x_add_cases)
+  apply (drule meta_mp)
+
+  
+   apply (linarith)
+  apply (drule meta_mp)
+   apply (meson nat_less_mult_monoish order_less_le_trans trans_less_add1)
+  apply (drule meta_mp, clarsimp)
+  apply (drule meta_mp, clarsimp)
+  apply (drule meta_mp, clarsimp)
+  
+   apply (meson add_mono_thms_linordered_semiring(2) diff_le_mono
+                div_le_mono dual_order.strict_iff_not dual_order.trans)
+  apply (drule meta_mp, clarsimp)
+   defer
+  apply (clarsimp)
+  sledgehammer
+
+  find_theorems name:induct "_ :: nat"
+  apply (induct n rule: less_induct)
+
+
+  apply (rule diff_lessE, assumption)
+  oops
+  apply (clarsimp simp: smt_arith_simplify)
+
+  apply (subgoal_tac "Suc (x + (x + x * x)) - n = Suc ((x + (x + x * x)) - n)")
+   apply (clarsimp)
+   apply (rule le_imp_less_Suc)
+
+   apply (insert x_add_cases[where x="x + n div x"])[1]
+   apply (elim disjE; clarsimp?)
+    apply (clarsimp simp: add.assoc[symmetric])
+  sledgehammer
+    apply (case_tac "n = 9 \<and> x = 9", clarsimp)
+
+    apply (rule order_trans)
+  apply (rule diff_le_mono2)
+    apply (case_tac "n = 9 \<and> x = 9", clarsimp)
+
+   apply (rule order_trans[rotated])
+    apply (rule diff_le_mono, assumption)
+   defer
+  using Suc_diff_le less_Suc_eq_le apply blast
+    apply (case_tac "n = 9 \<and> x = 4", clarsimp)
+
+   apply (insert x_add_cases[where x="x + n div x"])[1]
+   apply (elim disjE; clarsimp?)
+    apply (clarsimp simp: add.assoc[symmetric])
+  
+  apply (clarsimp simp: add.assoc, rule add_left_mono)
+  
+  apply (case_tac "n = 9 \<and> x = 4", clarsimp)
+
+    apply (subgoal_tac "n \<le> x + (x * x)")
+  
+  
+  apply (case_tac "n = 9 \<and> x = 3", clarsimp)
+  
+  
+  
+  
+
+lemma "unat (n :: 2 word) < unat (x + 1) * unat (x + 1) \<Longrightarrow> n < n + 1 \<Longrightarrow> x \<le> n \<Longrightarrow>
+       unat n < unat ((x + n div x) div 2 + 1) * unat ((x + n div x) div 2 + 1)" 
+  apply (erule diff_lessE)
+  apply (subgoal_tac "x + 1 \<noteq> 0")
+   apply (subst unatSuc2, clarsimp)+
+  apply (metis add_cancel_right_right bits_div_0 div_less_dividend_word less_is_non_zero_p1 one_add_one zero_neq_one)
+    apply (subst unatSuc2, clarsimp)+
+  apply (metis add_cancel_right_right bits_div_0 div_less_dividend_word less_is_non_zero_p1 one_add_one zero_neq_one)
+   apply (clarsimp)
+  oops
+   apply (unat_arith)
+   apply (clarsimp)
+   apply (safe)
+  nitpick
+  
+  find_theorems "unat (?x + ?y)"
+
+lemma (in hoare_logic) sqrt_le  : "sqrt' n \<le> n"
+  apply (induct rule: sqrt_induct)
+  by (metis (no_types, lifting) antisym_conv1 dual_order.strict_trans1 not_le_imp_less
+                                order_less_imp_le word_coorder.extremum_strict word_div_less)
+
+find_theorems name:helper
+
+thm square_less_than
+
+lemma (in hoare_logic) sqrt_le_eqI: "sqrt' n \<le> x \<Longrightarrow> x * x \<le> n \<Longrightarrow>  x * x div x = x \<Longrightarrow>  x = sqrt' n"
+  apply (rule sqrt_eqI[symmetric], clarsimp simp: sqrt_def)
+  by (metis order_le_less_trans sqrt_def sqrt_eqI sqrt_exists_uniquely)
+
+lemma div_2_helper: "na < na + 2 \<Longrightarrow> (2 + na :: u64) div 2 = 1 + (na div 2)"
+ 
+  by (simp add: add.commute div_helper)
+
+lemma " z \<noteq> 0 \<Longrightarrow> x \<noteq> 0 \<Longrightarrow> x < y div z \<longleftrightarrow> x * z < (y :: nat)"
+
+  find_theorems "?x < ?y div ?z \<longleftrightarrow> _"
+
+lemma "(x :: nat) < y \<Longrightarrow> x \<le> y \<and> x \<noteq> y"
+  sledgehammer
+  using nat_less_le by blast
+  using nless_le by blast
+  by fastforce
+
+
+find_theorems name:induct name:inc
+
+lemma midpoint_leI: "n div x \<le> x + 3 \<Longrightarrow>  ((x :: nat) + n div x) div 2 \<le> x + 1" 
+  by linarith
+
+lemma "x \<le> n \<Longrightarrow> n div x \<le> x + (y :: nat)"
+
+
+lemma midpoint_leD: " ((x :: nat) + n div x) div 2 \<le> x + 1 \<Longrightarrow> n div x \<le> x + 3 " 
+  by linarith
+
+lemma "Suc (na mod x) = x \<Longrightarrow> Suc na div x = Suc (na div x)"
+  by (meson div_Suc mod_Suc)
+
+lemma div_induct: "(\<And>k. k * (x :: nat) = n - (n mod x) \<Longrightarrow> P k) \<Longrightarrow> P (n div x)" 
+  by (metis minus_mod_eq_div_mult)
+
+lemma le_mul_mono: "x * y \<le> x * z \<Longrightarrow> x \<noteq> 0 \<Longrightarrow> y \<le> (z :: nat)"
+  by fastforce
+
+find_theorems "?x * ?y = ?y * ?x"
+
+lemma ge_sqrt_by_three:"(x + 1) * (x + 1) \<ge> n \<Longrightarrow> (n :: nat) div x \<le> x + 3"
+  apply (case_tac "x=0"; clarsimp)
+  apply (rule div_induct)
+  apply (rule le_mul_mono[where x=x])
+   apply (subst mult.commute)
+   apply (simp)
+proof -
+  fix k :: nat
+  assume a1: "k * x = n - n mod x"
+  assume a2: "n \<le> Suc (x + (x + x * x))"
+  have f3: "\<forall>n na nb. (n::nat) \<le> na + (n + nb)"
+    by simp
+  have f4: "n \<le> Suc (x * Suc (Suc x))"
+    using a2 by simp
+  have "\<forall>na. x * k \<le> na \<or> na < n"
+    using f3 a1 by (metis add.commute add_diff_inverse_nat minus_mod_eq_mult_div mod_div_decomp mult.commute)
+  then have "x * k \<le> x * (x + Suc (Suc 1))"
+    using f4 f3 by (smt (z3) Suc_eq_plus1 Suc_le_eq add.commute add_Suc_shift add_diff_inverse_nat less_Suc_eq_le linorder_not_less mult_Suc_right nat_add_left_cancel_le th2)
+  then show "n - n mod x \<le> x * (x + 3)"
+    using a1 by (smt (z3) One_nat_def Suc_eq_plus1 mult.commute numeral_2_eq_2 numeral_One numeral_plus_numeral semiring_norm(5))
+next
+  assume "0 < x"
+  then show "x \<noteq> 0"
+    by auto
+qed
+  
+  
+ 
+  
+lemma (in hoare_logic) "x \<le> (n :: u64) \<Longrightarrow> x < x + n div x \<Longrightarrow> x < x + 1 \<Longrightarrow>
+       (x + n div x) div 2 \<le> x + 1 \<Longrightarrow>
+       ((x + n div x) div 2 + n div ((x + n div x) div 2)) div 2 \<le> (x + n div x) div 2 + 1" 
+  apply (rule midpoint_leI)
+  apply (drule midpoint_leD)
+  apply (rule ge_sqrt_by_three)
+  apply (induct n rule: dec_induct)
+   apply (case_tac "x = 0"; clarsimp)
+   defer
+   apply (clarsimp simp: div_Suc split: if_splits)
+    apply (safe; clarsimp?)
+  
+  oops
+  apply (clarsimp simp: div_self)
+  find_theorems "?n div ?n"
+   apply (clarsimp)
+  apply (smt (verit, ccfv_SIG) add.right_neutral add_self_div_2 bits_div_by_0 div_le_dividend div_le_mono div_less div_self le_Suc_eq lessI midpoint_le)
+  apply (clarsimp)
+  apply (clarsimp simp: smt_arith_simplify ) 
+  sledgehammer
+  find_theorems "Suc ?x < ?y  \<longleftrightarrow> _"
+  apply (rule_tac x="1" in exI, clarsimp)
+  apply (safe; clarsimp?)
+  defer
+  
+  find_theorems "\<not> (?x \<le> ?y) \<longleftrightarrow> _"
+  apply (drule not_lessD)
+  find_theorems name:less_induct
+  apply (rule order_trans[where y= "x + 2"])
+   defer
+  
+  oops
+  apply (case_tac "x = n"; clarsimp)
+  apply (smt (verit, ccfv_SIG) add.commute add_le_same_cancel1 div_greater_zero_iff div_le_dividend le_SucI linorder_not_le midpoint_le order_trans plus_1_eq_Suc)
+  find_theorems name:mono name:mul name:le
+  find_theorems "?x div ?y \<le> ?z \<longleftrightarrow> _"
+  
+  
+  oops
+  apply (induct x rule:word_induct2; clarsimp)
+  apply (case_tac "1 + na = n"; clarsimp?)
+   apply (clarsimp simp: div_word_self)
+   apply (subst div_2_helper)
+    apply (metis add.commute add_diff_cancel2 word_leq_le_minus_one)
+
+   apply (subst div_2_helper)
+    apply (metis add.commute add_diff_cancel2 word_leq_le_minus_one)
+
+   apply (subst div_2_helper)
+    apply (metis add.commute add_diff_cancel2 word_leq_le_minus_one)
+  apply (smt (verit) add.assoc add.commute add_diff_cancel_left' antisym_conv1 bits_div_by_1 div_2_helper div_mod_step div_word_self dual_order.eq_iff even_add even_succ_div_2 le_m1_iff_lt le_no_overflow linorder_less_linear minus_mod_eq_mult_div mult_2 odd_iff_mod_2_eq_one one_add_one order_less_le word_eq_zeroI yet_another_helper)
+  apply (drule meta_mp)
+   apply (meson le_no_overflow lt1_neq0 olen_add_eqv word_coorder.extremum word_sub_mono2)
+  apply (drule meta_mp)
+   apply (metis add.commute word_overflow)
+  apply (drule meta_mp)
+   defer
+   apply (drule meta_mp)
+    defer
+    apply (drule meta_mp)
+  defer
+
+  sledgehammer
+  oops
+  apply (case_tac "x = 1 \<and> n = 6", clarsimp)
+
+lemma (in hoare_logic)" (\<And>n. hoare_triple (P n) (c n) Q) \<Longrightarrow> 
+   hoare_triple (\<lambda>s. n < n + 1 \<and> (n < n + 1 \<longrightarrow> P (sqrt' n) s))
+  (bindCont (integer_squareroot n) c) Q"
+  apply (case_tac "n = 0", clarsimp)
+  find_theorems name:induct "_ :: u64"
+  apply (rule hoare_weaken_pre)
+    apply (clarsimp simp: integer_squareroot_def)
+  apply (wp)
+    apply (clarsimp)
+  apply (clarsimp simp: integer_squareroot_aux.simps)
+
+  find_theorems bindCont name:assoc
+    apply (clarsimp simp: bind_assoc bindCont_return')
+
+  find_theorems re
+    apply (wp)
+   apply (clarsimp)
+  apply (rule hoare_weaken_pre)
+   apply (subst integer_squareroot_def )
+   apply (simp only: bindCont_assoc[symmetric] bindCont_return' Let_unfold)+
+   apply (rule wp)+
+   apply (simp only: bindCont_assoc[symmetric] bindCont_return')?
+
+
+  apply (rule 
+           integer_squareroot_aux_wp[where I="(\<lambda>x y n. y \<noteq> 0 \<and> y \<le> y + (n div y) \<and> x \<le> n 
+                                            \<and> x + 1 \<ge> y \<and> x \<ge> sqrt' n \<and>
+                                               y = (x + (n div x)) div 2 )"])
+  apply (wp)
+   apply (rule wp)
+   apply (rule wp)
+    apply (clarsimp)
+  apply (simp only: bindCont_assoc[symmetric] bindCont_return')?
+
+    apply (atomize)
+    apply (erule_tac x="fst (a, b)" in allE)
+    apply (subst (asm) fst_conv, assumption) 
+    apply (blast)
+  apply (clarsimp)
+  
+    apply (clarsimp, wp)[1]
+  apply (assumption)
+  apply (clarsimp)
+  apply (intro context_conjI impI allI; clarsimp?)+
+  apply (safe; clarsimp?)
+          apply (fastforce)
+  apply (metis (no_types, opaque_lifting) inc_i lt1_neq0 not_less_iff_gr_or_eq one_add_one word_le_less_eq word_less_div)
+                apply (smt (verit) add_diff_cancel_right' add_diff_eq diff_numeral_special(9) 
+div_helper div_mod_step mult_2 not_less_iff_gr_or_eq order_le_less sub_wrap_lt times_2_cases word_div_lt_eq_0 word_leq_minus_one_le)
+(*           apply (simp add: div_word_self)
+  using lt1_neq0 apply blast *)
+          apply (simp add: div_less_dividend_word less_is_non_zero_p1 word_le_less_eq)
+  apply (rule sqrt_le)
+  apply (erule word_sqrt_ge)
+  find_theorems sqrt'
+  apply (simp add: less_is_non_zero_p1 td_gal_lt unat_gt_0 unat_mono)
+         apply (simp add: div_less_dividend_word less_is_non_zero_p1 plus_one_helper)
+      apply (simp add: div_word_self)
+       apply (subgoal_tac "x = (sqrt' n)", clarsimp)
+       apply (rule sqrt_le_eqI, assumption)
+        apply (subgoal_tac " x = (x + n div x) div 2 \<or> x = (x + n div x) div 2 - 1")
+         apply (elim disjE)
+  using local.square_less_than apply fastforce
+  apply (metis leI le_div_timesI order_less_imp_le word_le_plus_either word_must_wrap yet_another_helper)
+     (*   apply (metis (no_types, lifting) diff_eq_eq le_step_down_word word_must_wrap) *)
+  
+  apply (metis (no_types, lifting) antisym_conv1 eq_diff_eq word_le_minus_one_leq word_must_wrap)
+
+  
+         apply (smt (z3) add.commute antisym_conv2 diff_add_cancel 
+                         div_less_dividend_word div_lt' div_to_mult_word_lt dual_order.strict_iff_not 
+                         eq_2_64_0 less_x_plus_1 mult_2 mult_2_right 
+                         one_add_one times_2_cases u64_max word_coorder.extremum_unique
+                         word_le_not_less word_plus_mcs_4 word_random x_square_defined_iff)
+    apply (metis (no_types, lifting) add_cancel_right_right le_step_down_word lt1_neq0 
+           mult_zero_right times_2_cases word_coorder.extremum_uniqueI word_less_1 word_less_div)
+  sledgehammer
+  apply (smt (verit, ccfv_SIG) add_cancel_left_right another_helper dual_order.order_iff_strict linorder_le_less_linear word_div_less word_le_plus_either)
+    apply force
+  defer
+  apply (meson another_helper word_le_plus_either word_sqrt_ge)
+  oops
+       
+
+end
+
+
+end
